src/group_action.lean
@@ -1,6 +1,63 @@
-import data.equiv group_theory.subgroup
+import data.equiv group_theory.coset
 
 universes u v w u₁
+
+namespace setoid
+variables {α : Sort u} [setoid α]
+
+lemma comm {a b : α} : a ≈ b ↔ b ≈ a :=
+⟨symm, symm⟩
+
+end setoid
+
+section coset_group
+variables {α : Type u} [group α] (s : set α) [is_subgroup s]
+variables (x y : α) (L : left_cosets s)
+
+local attribute [instance] left_rel
+
+def left_cosets.left_mul : left_cosets s :=
+quotient.lift_on L (λ z, ⟦x * z⟧) $ λ m n (H : m⁻¹ * n ∈ s),
+quotient.sound $ show (x * m)⁻¹ * (x * n) ∈ s, by simpa [mul_assoc]
+
+@[simp] lemma left_cosets.mul_eq :
+  left_cosets.left_mul s x ⟦y⟧ = ⟦x * y⟧ := rfl
+
+theorem left_cosets.one_mul :
+  left_cosets.left_mul s 1 L = L :=
+quotient.induction_on L $ λ _, by simp
+
+theorem left_cosets.mul_mul :
+  left_cosets.left_mul s (x * y) L
+  = left_cosets.left_mul s x (left_cosets.left_mul s y L) :=
+quotient.induction_on L $ λ _, by simp [mul_assoc]
+
+end coset_group
+
+namespace is_subgroup
+
+variables {α : Type u} [group α] (g x y : α) (s : set α) [is_subgroup s]
+
+def conjugate : set α :=
+{ x | g⁻¹ * x * g ∈ s }
+
+@[simp] lemma mem_conjugate_iff : x ∈ conjugate g s ↔ g⁻¹ * x * g ∈ s :=
+iff.refl _
+
+instance conjugate.is_subgroup : is_subgroup (conjugate g s) :=
+{ one_mem := have (1:α) ∈ s := is_submonoid.one_mem s, by simpa,
+  mul_mem := λ x y hx hy, have (g⁻¹ * x * g) * (g⁻¹ * y * g) ∈ s := is_submonoid.mul_mem hx hy,
+    by simpa [mul_assoc] using this,
+  inv_mem := λ x hx, have (g⁻¹ * x * g)⁻¹ ∈ s := is_subgroup.inv_mem hx,
+    by simpa [mul_assoc] using this }
+
+theorem conjugate_one : conjugate 1 s = s :=
+set.ext $ λ z, by simp
+
+theorem conjugate_mul : conjugate (x * y) s = conjugate x (conjugate y s) :=
+set.ext $ λ z, by simp [conjugate, mul_assoc]
+
+end is_subgroup
 
 variables (G : Type u) [group G] (X S : Type v)
 
@@ -29,6 +86,9 @@ eq.symm $ group_action.mul g h x
 lemma inv_act (H : g ● x = y) : g⁻¹ ● y = x :=
 by rw ← H; simp [act_act]
 
+lemma inv_act_iff : g⁻¹ ● y = x ↔ g ● x = y :=
+⟨λ H, by rw ← H; simp [act_act], inv_act⟩
+
 namespace group_action
 
 variables (G X g h x y)
@@ -53,16 +113,8 @@ def examples.mul_right_inv : group_action G G :=
 def examples.conjugate : group_action G G :=
 ⟨λ g x, g * x * g⁻¹, by simp, by simp [mul_assoc]⟩
 
-def examples.cosets (H : set G) (hs : is_subgroup H) : group_action G (cosets H) :=
-⟨λ g hH, ⟨(*) g '' hH.1, let ⟨h, hh⟩ := hH.2 in ⟨g * h,
-  by rw ← hh; apply set.ext; intro x; from
-  ⟨λ ⟨y, hyH, hghyx⟩, ⟨h * y, ⟨y, hyH, rfl⟩, by simpa [mul_assoc] using hghyx⟩,
-   λ ⟨y, ⟨z, hzH, hhzy⟩, hgyx⟩, ⟨z, hzH, by simp [mul_assoc, hhzy, hgyx]⟩⟩⟩⟩,
- λ gH, subtype.eq $ set.ext $ λ z, ⟨λ ⟨x, hx1, hx2⟩, by simp at hx2; rw ← hx2; from hx1,
-   λ h, ⟨z, h, by simp⟩⟩,
- λ g h rH, subtype.eq $ set.ext $ λ x,
-  ⟨λ ⟨y, hyH, hghyx⟩, ⟨h * y, ⟨y, hyH, rfl⟩, by simpa [mul_assoc] using hghyx⟩,
-   λ ⟨y, ⟨z, hzH, hhzy⟩, hgyx⟩, ⟨z, hzH, by simp [mul_assoc, hhzy, hgyx]⟩⟩⟩
+def examples.cosets (H : set G) (hs : is_subgroup H) : group_action G (left_cosets H) :=
+⟨left_cosets.left_mul H, left_cosets.one_mul H, left_cosets.mul_mul H⟩
 
 def examples.subsets : group_action G (set X) :=
 ⟨λ g A, (●) g '' A,
@@ -72,6 +124,11 @@ def examples.subsets : group_action G (set X) :=
  λ g h A, set.ext $ λ x,
   ⟨λ ⟨y, hyH, hghyx⟩, ⟨h ● y, ⟨y, hyH, rfl⟩, by simpa [mul_act] using hghyx⟩,
    λ ⟨y, ⟨z, hzH, hhzy⟩, hgyx⟩, ⟨z, hzH, by simp [mul_act, hhzy, hgyx]⟩⟩⟩
+
+def examples.subgroups : group_action G { s : set G // is_subgroup s } :=
+⟨λ g s, ⟨@is_subgroup.conjugate _ _ g s.1 s.2, @is_subgroup.conjugate.is_subgroup _ _ _ _ s.2⟩,
+ λ s, subtype.eq $ @is_subgroup.conjugate_one _ _ s.1 s.2,
+ λ g h s, subtype.eq $ @is_subgroup.conjugate_mul _ _ g h s.1 s.2⟩
 
 def examples.product : group_action G (G × S) :=
 ⟨λ g hx, (g * hx.1, hx.2), by simp, by simp [mul_assoc]⟩
@@ -101,8 +158,77 @@ def stab : set G :=
 
 @[simp] lemma mem_stab_iff : g ∈ stab G X x ↔ g ● x = x := iff.rfl
 
-def stab.is_subgroup : is_subgroup (stab G X x) :=
-⟨by simp, λ g h1 h h2, by simp [mul_act]; rw [inv_act h2]; simpa using h1⟩
+instance stab.is_subgroup : is_subgroup (stab G X x) :=
+{ mul_mem := λ g1 g2 hg1 hg2, by simp at hg1 hg2; simp [mul_act, hg1, hg2],
+  one_mem := by simp,
+  inv_mem := λ g hg, inv_act hg }
+set_option pp.proofs true
+set_option trace.check true
+
+def stab_cosets_to_orbit : left_cosets (stab G X x) → orbit G X x :=
+@quotient.lift _ _ (left_rel (stab G X x)) (λ g, (⟨g ● x, g, rfl⟩ : orbit G X x)) $
+λ g1 g2 (H : (g1⁻¹ * g2) ● x = x), subtype.eq $ inv_act_iff.1 $ eq.trans act_act H
+
+noncomputable def orbit_equiv_stab_cosets : orbit G X x ≃ left_cosets (stab G X x) :=
+equiv.symm $ @equiv.of_bijective _ _ (stab_cosets_to_orbit G X x) $
+⟨λ L1 L2, by letI := left_rel (stab G X x); exact
+  quotient.induction_on₂ L1 L2 (λ m n H,
+    have m ● x = n ● x, from subtype.mk.inj H,
+    quotient.sound $ show (m⁻¹ * n) ● x = x, by simpa [mul_act, inv_act_iff]),
+λ ⟨y, g, H⟩, by letI := left_rel (stab G X x); exact ⟨⟦g⟧, subtype.eq H⟩⟩
+
+noncomputable def orbit_stab : (orbit G X x × stab G X x) ≃ G :=
+(equiv.prod_congr (orbit_equiv_stab_cosets G X x) (equiv.refl $ stab G X x)).trans
+(is_subgroup.group_equiv_left_cosets_times_subgroup _).symm
+
+instance orbit_rel : setoid X :=
+⟨λ x y, ∃ g : G, g ● x = y,
+ λ x, ⟨1, by simp⟩,
+ λ x y ⟨g, H⟩, ⟨g⁻¹, by simp [inv_act_iff, H]⟩,
+ λ x y z ⟨g1, H1⟩ ⟨g2, H2⟩, ⟨g2 * g1, by simp [mul_act, H1, H2]⟩⟩
+
+def orbits : Type v := quotient (group_action.orbit_rel G X)
+
+def orbits_to_orbit : orbits G X → set X :=
+quotient.lift (orbit G X) $ λ x y ⟨g, H⟩,
+set.ext $ λ z,
+⟨λ ⟨g1, h1⟩, ⟨g1 * g⁻¹, by rw [mul_act, inv_act H, h1]⟩,
+ λ ⟨g1, h1⟩, ⟨g1 * g, by rw [mul_act, H, h1]⟩⟩
+
+theorem orbits_to_orbit_eq_orbit_out (A) : orbits_to_orbit G X A = orbit G X (quotient.out A) :=
+by rw [orbits_to_orbit, ← quotient.out_eq A, quotient.lift_beta]; simp
+
+theorem orbits_to_orbit_eq_fibre (A) : orbits_to_orbit G X A = { x | ⟦x⟧ = A } :=
+set.ext $ λ x, quotient.induction_on A $ λ z, by simp [orbits_to_orbit]; rw setoid.comm; refl
+
+theorem orbit_out_eq_fibre (A) : orbit G X (quotient.out A) = { x | ⟦x⟧ = A } :=
+(orbits_to_orbit_eq_orbit_out G X A).symm.trans (orbits_to_orbit_eq_fibre G X A)
+
+def stab_equiv (H : g ● x = y) : stab G X x ≃ stab G X y :=
+⟨λ g1, ⟨g * g1.1 * g⁻¹, by cases g1 with g1 h1; change g1 ● x = x at h1; simp [mul_act, inv_act H, h1, H]⟩,
+ λ g1, ⟨g⁻¹ * g1.1 * g, by cases g1 with g1 h1; change g1 ● y = y at h1; simp [mul_act, H, h1, inv_act H]⟩,
+ λ ⟨g1, h1⟩, by simp [mul_assoc],
+ λ ⟨g1, h1⟩, by simp [mul_assoc]⟩
+
+def fixed : set X := { x | g ● x = x }
+
+noncomputable def burnside : (Σ g, fixed G X g) ≃ (orbits G X × G) :=
+calc  (Σ g, fixed G X g)
+    ≃ (Σ x, stab G X x) :
+  ⟨λ z, ⟨z.2.1, z.1, z.2.2⟩, λ z, ⟨z.2.1, z.1, z.2.2⟩, λ ⟨g, x, h⟩, rfl, λ ⟨x, g, h⟩, rfl⟩
+... ≃ (Σ A : orbits G X, Σ x : { x | ⟦x⟧ = A }, stab G X x) :
+  ⟨λ z, ⟨⟦z.1⟧, ⟨_, rfl⟩, z.2⟩, λ z, ⟨z.2.1.1, z.2.2⟩, λ ⟨x, z⟩, rfl, λ ⟨A, ⟨x, (hx : ⟦x⟧ = A)⟩, z⟩, sigma.eq hx $ by subst hx⟩
+... ≃ (Σ A : orbits G X, Σ x : { x | ⟦x⟧ = A }, stab G X (quotient.out A)) :
+  equiv.sigma_congr_right (λ A, equiv.sigma_congr_right (λ ⟨x, (hx : ⟦x⟧ = A)⟩,
+    stab_equiv G X _ _ _ (classical.some_spec (quotient.exact (hx.trans (quotient.out_eq A).symm)))))
+... ≃ (Σ A : orbits G X, { x | ⟦x⟧ = A } × stab G X (quotient.out A)) :
+  equiv.sigma_congr_right (λ A, equiv.sigma_equiv_prod _ _)
+... ≃ (Σ A : orbits G X, orbit G X (quotient.out A) × stab G X (quotient.out A)) :
+  equiv.sigma_congr_right (λ A, by rw orbit_out_eq_fibre)
+... ≃ (Σ A : orbits G X, G) :
+  equiv.sigma_congr_right (λ A, orbit_stab G X _)
+... ≃ (orbits G X × G) :
+  equiv.sigma_equiv_prod _ _
 
 variables (Y : Type w) [group_action G Y]
 variables (Z : Type u₁) [group_action G Z]
